Veir/Dialects/LLZK/Include/OpInfo.lean
@@ -1,0 +1,76 @@
+module
+
+public import Veir.IR.Simp
+public import Veir.IR.OpInfo
+public import Veir.Verifier.Basic
+public import Veir.Dialects.LLZK.Include.Properties
+meta import Veir.Meta.OpCode
+
+namespace Veir
+
+public section
+
+@[opcodes]
+inductive Include_ where
+| from
+deriving Inhabited, Repr, Hashable, DecidableEq
+
+@[expose, properties_of]
+def Include_.propertiesOf (op : Include_) : Type :=
+match op with
+| .from => IncludeFromProperties
+
+def Include_.fromAttrDict
+    (op : Include_) (attrDict : Std.HashMap ByteArray Attribute) :
+    Except String (Include_.propertiesOf op) := by
+  cases op
+  exact IncludeFromProperties.fromAttrDict attrDict
+
+def Include_.toAttrDict
+    (op : Include_) (props : Include_.propertiesOf op) :
+    Std.HashMap ByteArray Attribute :=
+  match op with
+  | .from =>
+    ((Std.HashMap.emptyWithCapacity 2).insert
+      "sym_name".toUTF8 (Attribute.stringAttr props.sym_name)).insert
+      "path".toUTF8 (Attribute.stringAttr props.path)
+
+@[get_effects]
+def Include_.getEffects
+    (_op : Include_) (_props : Include_.propertiesOf _op) : MemoryEffects :=
+  .unknown
+
+def Include_.isConstantLike (_op : Include_) : Bool := false
+
+def Include_.hasSSADominance (_op : Include_) (_index : Nat) : Bool := true
+
+#generate_dialect Include_
+
+instance : IsOpCode Include_ where
+  fromName := Include_.fromName
+  name := Include_.name
+  propertiesOf := Include_.propertiesOf
+  fromAttrDict := Include_.fromAttrDict
+  toAttrDict := Include_.toAttrDict
+
+def Include_.verifyLocalInvariants {OpInfo : Type} [IsOpCode OpInfo]
+    [HasDialect OpInfo Include_] (opType : Include_) (op : OperationPtr)
+    (ctx : WfIRContext OpInfo) (opIn : op.InBounds ctx.raw) : Except String PUnit := do
+  match opType with
+  | .from => do
+    op.verifyPlainOpCounts ctx opIn 0 0
+    match op.getParentOp! ctx.raw with
+    | some parent =>
+      if IsOpCode.name (parent.getOpType! ctx.raw) ≠ "builtin.module".toUTF8 then
+        throw "include.from: Expected the parent operation to be a builtin.module"
+    | none => throw "include.from: Expected the parent operation to be a builtin.module"
+
+instance : HasOpInfo Include_ where
+  verifyLocalInvariants := Include_.verifyLocalInvariants
+  getEffects := Include_.getEffects
+  isConstantLike := Include_.isConstantLike
+  hasSSADominance := Include_.hasSSADominance
+
+end
+
+end Veir
