Test/Verifier/builtin_module_block_arguments.mlir
@@ -1,0 +1,6 @@
+// RUN: not veir-opt %s 2>&1 | filecheck %s
+
+// CHECK: builtin.module: Expected the body block to have 0 arguments
+"builtin.module"() ({
+^entry(%arg: i1):
+}) : () -> ()
