Test/Verifier/llzk_function_return_arity_mismatch.mlir
@@ -1,0 +1,8 @@
+// RUN: not veir-opt %s 2>&1 | filecheck %s
+
+// CHECK: function.return: Expected function.return to have 1 operand(s)
+"builtin.module"() ({
+  "function.def"() <{sym_name = "arity_mismatch", function_type = () -> !felt.type}> ({
+    "function.return"() : () -> ()
+  }) : () -> ()
+}) : () -> ()
